coq/Shared.v
@@ -14,25 +14,51 @@ Notation "'if' b 'then' v1 'else' v2" :=
 
 
 (**************************************************************)
+(** Auxiliary function to perform case analysis on an option 
+    without requiring an explicit match. *)
+
+Definition option_case {A B : Type} (d : B) (f : A -> B) (op : option A) : B :=
+  match op with
+  | None => d
+  | Some x => f x
+  end.
+
+
+(**************************************************************)
+(** ** Char-related functions *)
+
+(* Note that string is extracted to "char list" in Ocaml *)
+
+(* Int_of_char is currently directly extracted in Caml as:
+     "(fun c -> float_of_int (int_of_char c))". 
+   No property of this function is currently needed. *)
+
+Parameter int_of_char : Ascii.ascii -> int.
+
+(* Comparison on Ascii characters implemented as (=) on "char" in Caml *)
+
+Parameter ascii_compare : Ascii.ascii -> Ascii.ascii -> bool.
+Parameter ascii_compare_beq : forall (x y : Ascii.ascii),
+  (ascii_compare x y) <-> (x = y).
+
+Global Instance ascii_comparable : Comparable Ascii.ascii.
+Proof.
+  applys (comparable_beq ascii_compare).
+  applys ascii_compare_beq.
+Qed.
+
+(**************************************************************)
 (** ** String-related functions *)
 
-(* todo: extract in a more clever way ! *)
-Parameter int_of_char : Ascii.ascii -> int.
+(** Binding for Coq stdlib concatentation function *)
+
+Definition string_concat : string -> string -> string :=
+  String.append.
+
+(** Binding for Coq stdlib substring function *)
 
 Definition string_sub s (n l : int) : string :=
   substring (abs n) (abs l) s.
-
-Axiom ascii_compare : Ascii.ascii -> Ascii.ascii -> bool.
-
-Global Instance ascii_comparable : Comparable Ascii.ascii.
-Proof. applys (comparable_beq ascii_compare). skip. Qed. (* TODO:fix *)
-
-(* todo: implement using lib *)
-Parameter string_concat : string -> string -> string.
-
-(* MARTIN: is this used anywhere ? *)
-Parameter is_substring : string -> string -> Prop.
-Parameter is_substring_dec : forall s1 s2, Decidable (is_substring s1 s2).
 
 
 (**************************************************************)
@@ -48,99 +74,108 @@ Proof. introv. apply prove_Inhab. introv. auto*. Qed.
 
 
 (**************************************************************)
-(** ** Generalization of Pickable to function that return options *)
+(** ** POUR ARTHUR *)
 
-(* MARTIN: see whether it is possible to use Pickable directly *)
+(* Directly extract towards (<) in OCaml *)
 
-(** Pickable for option types *)
+Global Instance lt_int_decidable : forall i1 i2 : int, Decidable (i1 < i2).
+Admitted.
 
-Class Pickable_option (A : Type) (P : A -> Prop) := pickable_option_make {
-  pick_option : option A;
-  pick_option_correct : forall a, pick_option = Some a -> P a;
-  pick_option_defined : (exists a, P a) -> (exists a, pick_option = Some a) }.
-
-Implicit Arguments pick_option [A [Pickable_option]].
-Extraction Inline pick_option.
-
-Global Instance Pickable_option_Pickable : 
-  forall (A : Type) (P : A -> Prop), Inhab A -> (* todo: use `{Inhab A} *)
-  Pickable_option P -> Pickable P.
-Proof.
-  (* todo: clean up proof *)
-  introv I [[pi|] C D].
-   applys pickable_make pi. introv _. apply~ C.
-   applys pickable_make arbitrary. introv E. forwards (a&N): D E. inverts N.
-Qed.
-
-(** Application to LibHeap operation *)
-
-Require Import LibHeap.
-
-Global Instance binds_pickable_option : forall K V : Type,
-  `{Comparable K} -> `{Inhab V} ->
-  forall (h : heap K V) (v : K),
-  Pickable_option (binds h v).
-Proof.
-  introv CK IV; introv. applys pickable_option_make (read_option h v).
-   apply read_option_binds. 
-   introv [a Ba]. forwards R: @binds_read_option Ba. exists~ a.
-Qed.
-
-(**************************************************************)
-(** ** MARTIN: why do we need these? *)
-
-Axiom int_lt_dec : forall k1 k2 : int, Decidable (k1 < k2).
+(* Directly extract towards (<=) in OCaml *)
 
 Global Instance le_int_decidable : forall i1 i2 : int, Decidable (i1 <= i2).
 Admitted.
+(*
+Proof.
+  applys comparable_beq (fun i j => decide (i ?= j = Eq)). intros x y.
+  simpl; rew_refl; iff H; rewrite Z.compare_eq_iff in * |- *; inverts~ H.
+Qed.
+
+*)
+
+(* Directly extract towards (>=) in OCaml *)
 
 Global Instance ge_nat_decidable : forall n1 n2 : nat, Decidable (n1 >= n2).
 Admitted.
 
 
 
-(**************************************************************)
-(** ** MARTIN: do we still need this operation? Haven't we given it a better name? *)
-
-Definition morph_option {B C : Type} (c : C) (f : B -> C) (op : option B) : C :=
-  match op with
-  | None => c
-  | Some b => f b
-  end.
-
-(* MARTIN: does not seem to be used *)
-Definition unmonad_option {B : Type} (default : B) (op : option B) : B :=
-  morph_option default id op.
 
 
 (**************************************************************)
-(** ** MARTIN: where do we use this? *)
+(** ** MARTIN: where do we use this? 
+==> not used? *)
 
-Class FunctionalPred A (P:A->Prop) := functionalpred_make {
-    functional_pred : forall x y, P x -> P y -> x = y }.
+  Class FunctionalPred A (P:A->Prop) := functionalpred_make {
+      functional_pred : forall x y, P x -> P y -> x = y }.
 
-Global Instance apply_if_exists_pickable :
-  forall (A B : Type) (P : A -> Prop) (f : A -> B),
-  Pickable P -> FunctionalPred P ->
-  Pickable (fun v => exists x, P x /\ f x = v).
-Proof.
-  introv [p Hp] [F]. applys pickable_make (f p).
-  intros (a & x & (Hx & Ha)). exists x. splits~.
-  forwards*: F Hx Hp. substs~.
-Qed.
+  Global Instance apply_if_exists_pickable :
+    forall (A B : Type) (P : A -> Prop) (f : A -> B),
+    Pickable P -> FunctionalPred P ->
+    Pickable (fun v => exists x, P x /\ f x = v).
+  Proof.
+    introv [p Hp] [F]. applys pickable_make (f p).
+    intros (a & x & (Hx & Ha)). exists x. splits~.
+    forwards*: F Hx Hp. substs~.
+  Qed.
 
-Global Instance binds_functionnal : forall (H K : Type) (h : heap H K) k,
-  Comparable H -> Inhab K ->
-  FunctionalPred (binds h k).
-Proof. introv C I. applys functionalpred_make. apply binds_func. Qed.
-(* End of this little test. *)
+  Require Import LibHeap.
+  Global Instance binds_functionnal : forall (H K : Type) (h : heap H K) k,
+    Comparable H -> Inhab K ->
+    FunctionalPred (binds h k).
+  Proof. introv C I. applys functionalpred_make. apply binds_func. Qed.
+  (* End of this little test. *)
+
+
+
+
+(**************************************************************)
+(** ** Generalization of Pickable to function that return options 
+==> not used?  *)
+
+  (* MARTIN: see whether it is possible to use Pickable directly *)
+
+  (** Pickable for option types *)
+
+  Class Pickable_option (A : Type) (P : A -> Prop) := pickable_option_make {
+    pick_option : option A;
+    pick_option_correct : forall a, pick_option = Some a -> P a;
+    pick_option_defined : (exists a, P a) -> (exists a, pick_option = Some a) }.
+
+  Implicit Arguments pick_option [A [Pickable_option]].
+  Extraction Inline pick_option.
+
+  Global Instance Pickable_option_Pickable : 
+    forall (A : Type) (P : A -> Prop), Inhab A -> (* todo: use `{Inhab A} *)
+    Pickable_option P -> Pickable P.
+  Proof.
+    (* todo: clean up proof *)
+    introv I [[pi|] C D].
+     applys pickable_make pi. introv _. apply~ C.
+     applys pickable_make arbitrary. introv E. forwards (a&N): D E. inverts N.
+  Qed.
+
+  (** Application to LibHeap operation *)
+
+  Require Import LibHeap.
+
+  Global Instance binds_pickable_option : forall K V : Type,
+    `{Comparable K} -> `{Inhab V} ->
+    forall (h : heap K V) (v : K),
+    Pickable_option (binds h v).
+  Proof.
+    introv CK IV; introv. applys pickable_option_make (read_option h v).
+     apply read_option_binds. 
+     introv [a Ba]. forwards R: @binds_read_option Ba. exists~ a.
+  Qed.
+
 
 
 (**************************************************************)
 
-(* MARTIN: modifier l'interpréteur
+(* MARTIN: modifier l'interpreteur
   pour utiliser une fonction qui fasse 
-  last et removelast en même temps:
+  last et removelast en meme temps:
   cf.   LibList.take_drop_last.
   
   Ensuite, supprimer le lemme ci-dessous *)
@@ -156,9 +191,27 @@ Proof.
 Qed.
 
 
+(* MARTIN:
+  by the way, please rename rule red_spec_arguments_object_map_3_cont_skip
+  so that it does not contain the word "skip" (use "next" or something else).
+*)
+
+(* MARTIN:
+   resoudre les skips de Global Instance object_properties_keys_as_list_pickable_option
+   dans JsCorrectness
+
+  Dans run_call_prealloc_correct,
+  remplacer les "skip" par "discriminate": je crois que ca suffit pour 
+   resoudre le but, puisqu'on a un result_out egal a un result_unimplemented
+   dans le contexte.;
+  
+  Dans JSNumber, reparer:  Global Instance number_comparable : Comparable number.
+
+*)
 (**************************************************************)
-(** ** MARTIN: remplacer "In" par "Mem",; 
-   J'ai ajouté Mem_decidable. On pourra alors supprimer les defs ci dessous *)
+(** ** MARTIN: TODO remplacer "In" par "Mem",; 
+   J'ai ajoute Mem_decidable dans LibList.v.
+   On peut donc supprimer les defs ci dessous *)
 
 Fixpoint mem_decide (A : Type) `{Comparable A} (x : A) (l : list A) :=
   match l with
@@ -197,8 +250,9 @@ Qed.
 (***********************************************************)
 (** * Heap with a counter for allocating fresh locations *)
 
-(* MARTIN: j'ai du mal à comprendre comment ça peut marcher. *)
+(* TODO: remove this if not needed. *)
 
+Require Import LibHeap.
 Module HeapGen (Export Heap : HeapSpec) : HeapSpec.
 Generalizable Variable K V.
 
