coq/bin.v
@@ -1,0 +1,164 @@
+(* Already there, but didn't work as instance... *)
+Global Instance prod_inhab : forall A B : Type,
+  Inhab A -> Inhab B ->
+  Inhab (A * B).
+Proof.
+  introv IA IB.
+  destruct IA. destruct inhabited as [a _].
+  destruct IB. destruct inhabited as [b _].
+  applys prove_Inhab (a, b).
+Qed.
+
+
+Ltac decompose_base X I :=
+  gen ltac_mark; gen X; intros X;
+  let Y := fresh in set (Y:=X); destruct X as I; rename Y into X;
+  intro_until_mark.
+
+Tactic Notation "decompose" ident(E) "as" simple_intropattern(I) :=
+  decompose_base E I.
+
+
+(**************************************************************)
+(** **  *)
+
+(* should follow from Incl order:
+Section Instances.
+Variables (A:Type).
+Global Instance set_incl_union_l :
+  Incl_refl (T:=set A).
+Admitted.
+Global Instance set_incl_refl :
+  Incl_trans (T:=set A).
+Admitted.
+End Instances.
+*)
+
+(* not used:
+Lemma union_idem_r : forall A (E F:set A),
+  E \u F \u F = E \u F.
+Admitted.
+*)
+
+(* not used:
+Lemma subset_inter_weak_l : forall {A : Type} (E F : fset A),
+  FsetImpl.subset (FsetImpl.inter E F) E.
+Proof. intros_all. rewrite FsetImpl.in_inter in H. auto*. Qed.
+
+Lemma subset_inter_weak_r : forall {A : Type} (E F : fset A),
+  FsetImpl.subset (FsetImpl.inter E F) F.
+Proof. intros_all. rewrite FsetImpl.in_inter in H. auto*. Qed.
+*)
+
+
+(**************************************************************)
+
+(* MARTIN: check where it is used ? 
+   it's not clear why we'd ever need to compare propositions...:
+   *)
+Global Instance eq_prop_decidable : forall (P Q : Prop),
+  Decidable P -> Decidable Q ->
+  Decidable (P = Q). 
+Proof.
+  introv [p Hp] [q Hq]. applys decidable_make (decide (p = q)).
+  skip. (* TODO : complete proof *)
+Qed.
+
+
+Lemma option_apply_some_back : forall (A B : Type) (f : A -> option B) ao (b : B),
+                                 LibOption.apply f ao = Some b ->
+                                 exists a, ao = Some a /\ f a = Some b.
+Proof.  introv E. destruct~ ao. exists a. splits~. inverts~ E. Qed.
+
+Lemma option_apply_some_forw : forall (A B : Type) (f : A -> option B) ao (a:A) (b:B),
+  ao = Some a ->
+  f a = Some b ->
+  LibOption.apply f ao = Some b.
+Proof. introv E1 E2. substs. unfold apply. apply E2. Qed.
+
+
+
+Definition hd_inhab {A : Type} `{Inhab A} (l : list A) : A :=
+  match l with
+  | nil => arbitrary
+  | a :: l' => a
+  end.
+
+Fixpoint map_nth {A B : Type} (d : B) (f : A -> B) (i : nat) (s : list A) : B :=
+  match i, s with
+  | O, a :: _ => f a
+  | S i', _ :: s' => map_nth d f i' s'
+  | _, _ => d
+  end.
+
+Definition get_nth {A : Type} (d : A) (i : nat) (s : list A) : A :=
+  map_nth (fun _ : unit => d) (fun (x : A) _ => x) i s tt.
+
+Lemma get_nth_nil : forall (A : Type) (d : A) (i : nat),
+  get_nth d i nil = d.
+Proof. introv. destruct~ i. Qed.
+
+Lemma get_nth_null : forall (A : Type) (d a : A) (s : list A),
+  get_nth d 0 (a :: s) = a.
+Proof. introv. reflexivity. Qed.
+
+Lemma get_nth_cons : forall (A : Type) (i : nat) (d a : A) (s : list A),
+  get_nth d (S i) (a :: s) = get_nth d i s.
+Proof. introv. reflexivity. Qed.
+
+(** [list_get_last ls] returns [None] if the list given is empty
+    or [Some (ls',x)] where [ls=ls'++x::nil] otherwise. *)
+
+Fixpoint lib_get_last (A:Type) (ls:list A) : option (list A * A) :=
+  match ls with
+  | nil => None
+  | a::ls' =>
+    match ls' with
+    | nil => Some (nil,a)
+    | _ => LibOption.map (fun p => let '(ls',x) := p in (a::ls',x)) (lib_get_last ls')
+    end
+  end.
+
+Lemma lib_get_last_spec : forall (A:Type) (ls:list A),
+  match lib_get_last ls with
+  | None => (ls = nil)
+  | Some (ls',x) => (ls = LibList.append ls' (x::nil))
+  end.
+Proof.
+  intros. induction ls; simpl.
+  auto.
+  destruct ls as [|b ls].
+    rew_list*.
+    destruct (lib_get_last (b::ls)) as [(?&?)|]; simpls.
+      rew_list*. congruence.
+      congruence.
+Qed.
+
+Lemma lib_get_last_nil : forall (A:Type),
+  lib_get_last (@nil A) = None.
+Proof. auto. Qed.
+
+Lemma lib_get_last_cons : forall (A:Type) ls,
+  ls <> nil -> exists (x:A) (ls':list A),
+     lib_get_last ls = Some (ls',x) 
+  /\ ls = LibList.append ls' (x::nil).
+Proof. 
+  intros. lets M: (lib_get_last_spec ls).
+  destruct (lib_get_last ls) as [(ls'&x)|]. 
+    subst. exists* x ls'.
+    false.
+Qed.
+
+
+
+(* MARTIN: is this used anywhere ? *)
+Parameter is_substring : string -> string -> Prop.
+Parameter is_substring_dec : forall s1 s2, Decidable (is_substring s1 s2).
+
+Axiom int_lt_dec : forall k1 k2 : int, Decidable (k1 < k2).
+Extract Constant int_lt_dec => "(<)".
+
+
+(* MARTIN: does not seem to be used *)
+Definition unmonad_option {B : Type} (default : B) (op : option B) : B :=
+  option_case default id op.
